Some correctness proofs

Strings.thy
@@ -16,29 +16,81 @@ Pure string predicates are defined in "strings/Words", regular expression in "st
 
 abbreviation str_concat:: "'a word \<Rightarrow> 'a word  \<Rightarrow> 'a word"  where "(str_concat) u v \<equiv> u@v" 
 abbreviation str_len:: "'a word \<Rightarrow> int" where  "str_len w \<equiv> of_nat (length w)"
-abbreviation str_at:: "'a word \<Rightarrow> int \<Rightarrow> 'a word" where "str_at w i \<equiv> (at w (nat i))"
 
-abbreviation str_substr:: "'a word \<Rightarrow> int \<Rightarrow> int \<Rightarrow> 'a word"  where "str_substr w i n \<equiv> if (n < 0 \<or> i<0 \<or> ((nat i) \<ge> (length w))) then \<epsilon> else  fac w (nat i) (nat n)"
 
-lemma [simp]: "(n < 0 \<or> i<0 \<or> ((nat i) \<ge> (length w))) \<Longrightarrow> str_substr w i n =  \<epsilon>"
+abbreviation str_at:: "'a word \<Rightarrow> int \<Rightarrow> 'a word" where "str_at w i \<equiv> if i \<ge> 0 then (at w (nat i)) else \<epsilon>"
+abbreviation str_substr:: "'a word \<Rightarrow> int \<Rightarrow> int \<Rightarrow> 'a word"  where "str_substr w m n \<equiv> if (n \<ge> 0 \<and> 0\<le>m \<and> ((nat m) \<le> (length w)-1)) then  fac w (nat m) (nat n) else \<epsilon>"
+
+(* Correctness of at: \<lbrakk>str.at\<rbrakk>(w, n) = \<lbrakk>str.substr\<rbrakk>(w, n, 1) *)
+theorem at_correct: "str_at w n = str_substr w n 1"
+  unfolding fac_def at_def
   apply(auto)
-  done
+  by (metis (no_types, lifting) append.simps(2) append_take_drop_id first.simps(1) first.simps(2) take_Suc take_eq_Nil2)
 
-lemma [simp]: "\<not>(n < 0 \<or> i<0 \<or> ((nat i) \<ge> (length w))) \<Longrightarrow> str_substr w i n = fac w (nat i) (nat n)"
-  apply(auto)
-  done
+
+(* Correctness of substr: 
+   - \<lbrakk>str.substr\<rbrakk>(w, m, n) is the unique word v such that
+     for some words x and y
+      - w = xvy
+      - |x| = m
+      - |y| = min(n, |w| - m) 
+                                    if 0 <= m < |w| and 0 < n
+    - \<lbrakk>str.substr\<rbrakk>(w, m, n) = \<epsilon>      otherwise
+*)
+theorem substr_correct1: 
+  fixes m::"int" and n::"int"
+  shows "0\<le>m \<and> m < (int (length w)) \<and> 0 < n \<Longrightarrow> (str_substr w m n = v \<Longrightarrow> (EX x y. (w = x@v@y \<and> ((int (length x)) = m) \<and> (int (length v)) = (min n ((int (length w)) - m)))))"
+  unfolding fac_def
+  apply(auto)+
+  apply(simp add: int_eq_iff min_def)+
+  apply(auto simp add:  int_ops(6) le_nat_iff)+
+   apply (metis append.right_neutral append_take_drop_id le_nat_iff length_take less_le_not_le min_def nat_diff_distrib nat_int)
+  by (smt (verit, best) append_take_drop_id le_nat_iff length_take min_def)
+
+theorem substr_correct2:
+fixes m::"int" and n::"int"
+shows "\<not>(0\<le>m \<and> m < (int (length w)) \<and> 0 < n) \<Longrightarrow> (str_substr w m n = \<epsilon>)"
+  unfolding fac_def by auto
+  
 
 abbreviation str_prefixof:: "'a word \<Rightarrow> 'a word \<Rightarrow> bool" where "str_prefixof \<equiv> Words.is_prefix"
 abbreviation str_suffixof:: "'a word \<Rightarrow> 'a word \<Rightarrow> bool" where "str_suffixof \<equiv> Words.is_suffix"
+
+(* Correctness of prefixof: \<lbrakk>str.prefixof\<rbrakk>(v, w) = true iff w = vx₂ for some word x *)
+theorem prefixof_correct: "str_prefixof v w \<longleftrightarrow> (EX x. w = v@x)"
+  unfolding is_prefix_def
+  apply(auto)
+  by (metis append_take_drop_id)
+
+(* Correctness of suffixof: \<lbrakk>str.suffixof\<rbrakk>(v, w) = true iff w = xv₂ for some word x *)
+theorem suffix_correct: "str_suffixof v w \<longleftrightarrow> (EX x. w = x@v)"
+  unfolding  is_suffix_def is_prefix_def
+  apply(auto)
+  by (metis append_take_drop_id rev_append rev_rev_ident)
+
 abbreviation str_contains:: "'a word \<Rightarrow> 'a word \<Rightarrow> bool" where "str_contains \<equiv> Words.contains"
+
+(* Correctness of contains: \<lbrakk>str.contains\<rbrakk>(w, v) = true  iff  w = xvy₃ for some words x,y*)
+theorem contain_correct: "Words.contains w v \<longleftrightarrow>(EX x y. w = x@v@y)"
+  apply(induct w)
+   apply(simp)
+  apply(auto simp add: Strings.prefixof_correct)
+     apply (metis append_Cons)
+    apply (metis append_Cons)
+   apply (metis append_Nil)
+  by (metis append_eq_Cons_conv)
+  
 
 abbreviation str_indexof:: "'a word \<Rightarrow> 'a word \<Rightarrow> int \<Rightarrow> int" 
   where "str_indexof h n s \<equiv> if s \<ge> 0 then (case find (drop (nat s) h) n of Some r \<Rightarrow> (int r) | option.None \<Rightarrow> -1) else (-1)"
 
 (* Regular Expression Functions *)
 
-abbreviation str_to_re:: "'a word \<Rightarrow> 'a regex" where "str_to_re w \<equiv> regex.Const w"
 abbreviation str_in_re:: "'a word \<Rightarrow> 'a regex \<Rightarrow> bool" where "str_in_re w R \<equiv> contains w R"
+
+
+
+abbreviation str_to_re:: "'a word \<Rightarrow> 'a regex" where "str_to_re w \<equiv> regex.Const w"
 abbreviation re_none:: "'a regex" where "re_none \<equiv> regex.None"
 abbreviation re_allchar:: "'a regex" where "re_allchar \<equiv> regex.Any"
 (* missing:  re_all*)
