Core.thy
@@ -2,14 +2,14 @@ theory Core
   imports Main
 begin
 
-abbreviation ite:: "bool \<Rightarrow> 's \<Rightarrow> 's \<Rightarrow> 's" where "ite a B C  \<equiv> if a then B else C"
+definition ite:: "bool \<Rightarrow> 's \<Rightarrow> 's \<Rightarrow> 's" where "ite a B C  \<equiv> if a then B else C"
 
 lemma ite_true[simp]: "(ite a B C) \<and> a \<Longrightarrow> B"
-  apply(simp)
+  apply(simp add: ite_def)
   done
 
 lemma ite_false[simp]: "(ite a B C) \<and> \<not> a \<Longrightarrow> C"
-  apply(simp)
+  apply(simp add: ite_def)
   done
 
 end
